src/axioms.v
@@ -5,7 +5,7 @@ From spacelambda Require Import wp_all wp_closure wp_adequacy.
 
 Print Assumptions wp_adequacy.
 Print Assumptions wp_alloc.
-Print Assumptions wp_bin_op.
+Print Assumptions wp_call_prim.
 Print Assumptions wp_call.
 Print Assumptions wp_mk_clo.
 Print Assumptions wp_call_clo.
